inhale works

src/main/scala/viper/carbon/modules/HeapModule.scala
@@ -151,7 +151,7 @@ trait HeapModule extends Module with CarbonStateComponent {
 
   def currentHeap:Seq[Exp]
 
-  def identicalOnKnownLocations(heap:Seq[Exp],mask:Seq[Exp]):Exp
+  def identicalOnKnownLocations(heap:Seq[Exp],mask:Seq[Exp], bmask:Seq[Exp]):Exp
 
   /**
     * Adds assumption that current heap equals heap represented by s
